Impl and prove movbe elim correct, under cpuid assumption. See msg.
Previously, when we implemented the movbe elimination
transformation, the semantics of movbe weren't actually sound. This
was because there was no CPUID check on them. Since then, I noticed
that this can cause programs to crash on certain CPUs (which indeed
led to the movbe elimination transform), and since then, the CPUID
check was added.

Due to the addition of this check, we actually need to relax our
statement of correctness of this transformation. In particular, we
need to ensure that the transformation handles this CPUID check
correctly, rather than simply assuming that it is correct. The plan is
to fix this up in some upcoming commits.

vale/code/lib/transformers/Vale.Transformers.MovbeElim.fst
@@ -11,12 +11,103 @@ open Vale.X64.InsLemmas
 
 open Vale.Transformers.PeepHole
 
-let movbe_elim_ph (is:list ins) : Tot (option (list ins)) =
-  None (* Safe, but currently behaves as a no-op due to this *)
+let movbe_elim_input_hint : pos = 1
 
+let movbe_elim_ph (is:list ins) : Tot (option (list ins)) =
+  match is with
+  | [Instr i oprs (AnnotateMovbe64 proof_of_movbe)] ->
+    let oprs:normal (instr_operands_t [out op64] [op64]) =
+      coerce_to_normal #(instr_operands_t [out op64] [op64]) oprs in
+    let (dst, (src, ())) = oprs in
+    if OReg? dst then (
+      let mov = make_instr ins_Mov64 dst src in
+      let bswap = make_instr ins_Bswap64 dst in
+      Some [mov; bswap]
+    ) else None
+  | _ -> None
+
+module T = Vale.Def.Types_s
+module H = Vale.Arch.Heap
+
+#push-options "--z3rlimit 10 --initial_fuel 0 --max_fuel 0 --initial_ifuel 2 --max_ifuel 2"
+let lemma_update_to_valid_destination_keeps_it_as_valid_src (o:operand64) (s:machine_state) (v:nat64) :
+  Lemma
+    (requires (valid_dst_operand64 o s))
+    (ensures (
+        let s' = update_operand64_preserve_flags'' o v s s in
+        valid_src_operand64_and_taint o s' /\
+        eval_operand o s' == v)) =
+  reveal_opaque (`%valid_addr64) valid_addr64;
+  update_heap64_reveal ();
+  get_heap_val64_reveal ()
+#pop-options
+
+#push-options "--z3rlimit 10 --initial_fuel 0 --max_fuel 0 --initial_ifuel 1 --max_ifuel 1"
+let lemma_double_update_reg (dst:operand64) (s0 s1 s2 s3:machine_state) (v v_fin:nat64) :
+  Lemma
+    (requires (
+        (OReg? dst) /\
+        (valid_dst_operand64 dst s0) /\
+        (s1 == update_operand64_preserve_flags'' dst v s0 s0) /\
+        (s2 == update_operand64_preserve_flags'' dst v_fin s1 s1) /\
+        (s3 == update_operand64_preserve_flags'' dst v_fin s0 s0)))
+    (ensures (
+        equiv_states s2 s3)) =
+  match dst with
+  | OReg r -> assert (equiv_states_ext s2 s3) (* OBSERVE *)
+#pop-options
+
+#push-options "--initial_fuel 2 --max_fuel 2 --initial_ifuel 0 --max_ifuel 0"
+let lemma_movbe_is_mov_bswap (dst src:operand64) (s:machine_state) :
+  Lemma
+    (requires (OReg? dst))
+    (ensures (
+        let movbe = make_instr_annotate ins_MovBe64 (AnnotateMovbe64 ()) dst src in
+        let mov = make_instr ins_Mov64 dst src in
+        let bswap = make_instr ins_Bswap64 dst in
+        equiv_states_or_both_not_ok
+          (machine_eval_ins movbe s)
+          (machine_eval_ins bswap (machine_eval_ins mov s)))) =
+  let movbe = make_instr_annotate ins_MovBe64 (AnnotateMovbe64 ()) dst src in
+  let mov = make_instr ins_Mov64 dst src in
+  let bswap = make_instr ins_Bswap64 dst in
+  let s_movbe = machine_eval_ins movbe s in
+  let s_mov = machine_eval_ins mov s in
+  let s_bswap = machine_eval_ins bswap s_mov in
+  if valid_src_operand64_and_taint src s && valid_dst_operand64 dst s then (
+    let src_v = eval_operand src s in
+    let dst_movbe_v = T.reverse_bytes_nat64 src_v in
+    let dst_mov_v = eval_operand dst s_mov in
+    let dst_bswap_v = T.reverse_bytes_nat64 dst_mov_v in
+    assume (Vale.X64.CPU_Features_s.movbe_enabled);
+    assert (s_movbe == update_operand64_preserve_flags'' dst dst_movbe_v s s); // this fails now, because there is a "movbe_enabled" check on movbe
+    assert (s_mov == update_operand64_preserve_flags'' dst src_v s s);
+    lemma_update_to_valid_destination_keeps_it_as_valid_src dst s src_v;
+    assert (eval_operand dst s_mov == src_v);
+    assert (valid_src_operand64_and_taint dst s_mov);
+    assert (s_bswap == update_operand64_preserve_flags'' dst dst_bswap_v s_mov s_mov);
+    assert (src_v == dst_mov_v);
+    assert (dst_movbe_v == dst_bswap_v);
+    lemma_double_update_reg dst s s_mov s_bswap s_movbe src_v dst_bswap_v
+  ) else (
+    assert (s_movbe == {s with ms_ok = false});
+    assert (s_mov == {s with ms_ok = false});
+    assert (s_bswap.ms_ok == false)
+  )
+#pop-options
+
+#push-options "--initial_fuel 3 --max_fuel 3 --initial_ifuel 0 --max_ifuel 0"
 let movbe_elim_correct (is:list ins) (s:machine_state) :
   Lemma (peephole_correct movbe_elim_ph is s)
     [SMTPat (peephole_correct movbe_elim_ph is s)] =
-  ()
-
-let movbe_elim_input_hint : pos = 1
+  match is with
+  | [Instr i oprs (AnnotateMovbe64 proof_of_movbe)] ->
+    let oprs:normal (instr_operands_t [out op64] [op64]) =
+      coerce_to_normal #(instr_operands_t [out op64] [op64]) oprs in
+    let (dst, (src, ())) = oprs in
+    if OReg? dst then (
+      let Some is' = movbe_elim_ph is in
+      lemma_movbe_is_mov_bswap dst src s
+    ) else ()
+  | _ -> ()
+#pop-options
